

Vector Calculus

①

Que 1) Find the directional derivative of $f(x, y, z) = xy^2 + yz^3$ at the point $(2, -1, 1)$ in the direction of vector $\mathbf{i} + 2\mathbf{j} + 2\mathbf{k}$.

Soln

Given that

$$f(x, y, z) = xy^2 + yz^3 \quad \text{--- (1)}$$

let \vec{d} be the vector. Then

$$\vec{d} = \mathbf{i} + 2\mathbf{j} + 2\mathbf{k}$$

$$\text{Now } \nabla f = \mathbf{i} \frac{\partial}{\partial x} (xy^2 + yz^3) + \mathbf{j} \frac{\partial}{\partial y} (xy^2 + yz^3) + \mathbf{k} \frac{\partial}{\partial z} (xy^2 + yz^3)$$

$$\nabla f = \mathbf{i} (y^2) + \mathbf{j} (2xy + z^3) + \mathbf{k} (3z^2y)$$

$$\text{At } (2, -1, 1)$$

$$\nabla f = \mathbf{i} - 3\mathbf{j} - 3\mathbf{k}$$

directional derivative of f in direction of vector $\vec{d} = \nabla f \cdot \hat{d}$

$$= \nabla f \cdot \frac{\vec{d}}{|\vec{d}|} = (\mathbf{i} - 3\mathbf{j} - 3\mathbf{k}) \cdot \frac{(\mathbf{i} + 2\mathbf{j} + 2\mathbf{k})}{\sqrt{1+4+4}}$$

$$= \frac{1-6-6}{3} = \frac{-11}{3}$$

Que) What is the directional derivative of $\phi = xy^2 + yz^3$ at the point $(2, -1, 1)$ in the direction of the normal to the surface $x \log z - y^2 = -4$ at $(-1, 2, 1)$

Soln - Given surface is

$$\phi = xy^2 + yz^3 \quad \text{--- (1)}$$

and

$$f \equiv x \log z - y^2 + 4 = 0 \quad \text{--- (2)}$$

$$\nabla \phi = \mathbf{i} \frac{\partial}{\partial x} (xy^2 + yz^3) + \mathbf{j} \frac{\partial}{\partial y} (xy^2 + yz^3) + \mathbf{k} \frac{\partial}{\partial z} (xy^2 + yz^3)$$

$$= \mathbf{i} (y^2) + \mathbf{j} (2xy + z^3) + \mathbf{k} (3z^2y)$$

$$\text{At } (2, -1, 1)$$

$$\nabla \phi = \mathbf{i} + \mathbf{j} (-4 + 1) + \mathbf{k} (-3)$$

$$\nabla \phi = \mathbf{i} - 3\mathbf{j} - 3\mathbf{k}$$

Now

$$\nabla f = \mathbf{i} \frac{\partial}{\partial x} (x \log z - y^2 + 4) + \mathbf{j} \frac{\partial}{\partial y} (x \log z - y^2 + 4) + \mathbf{k} \frac{\partial}{\partial z} (x \log z - y^2 + 4)$$

(2)

$$\nabla f = \mathbf{i} (\log z) + \mathbf{j} (-2y) + \mathbf{k} \left(\frac{2x}{z} \right)$$

$$\text{At } (-1, 2, 1)$$

$$\nabla f = \mathbf{i} \log 1 + \mathbf{j} (-4) + \mathbf{k} \left(\frac{-2}{1} \right)$$

$$\nabla f = 0\mathbf{i} - 4\mathbf{j} - \mathbf{k}$$

~~let \vec{v}~~

Direction derivative of ϕ in the direction of normal to the surface f

$$= \nabla \phi \cdot \frac{\nabla f}{|\nabla f|}$$

$$= (\mathbf{i} - 3\mathbf{j} - 3\mathbf{k}) \cdot \frac{(0\mathbf{i} - 4\mathbf{j} - \mathbf{k})}{\sqrt{0+16+1}}$$

$$= \frac{0+12+3}{\sqrt{17}} = \frac{15}{\sqrt{17}}$$

Que) Find the angle between the surfaces $x^2+y^2+z^2=9$ and ~~z~~ $z=x^2+y^2-3$ at the point $(2, -1, 2)$

Soln — let $f_1 \equiv x^2+y^2+z^2-9=0$
 $f_2 \equiv x^2+y^2-z-3=0$

Then

$$N_1 = \nabla f_1 = 2x\mathbf{i} + 2y\mathbf{j} + 2z\mathbf{k}$$

$$\text{At } (2, -1, 2)$$

$$N_1 = 4\mathbf{i} - 2\mathbf{j} + 4\mathbf{k}$$

$$N_2 = \nabla f_2 = 2x\mathbf{i} + 2y\mathbf{j} - \mathbf{k}$$

$$\text{At } (2, -1, 2)$$

$$N_2 = 4\mathbf{i} - 2\mathbf{j} - \mathbf{k}$$

Since the angle θ between the two surfaces at a point is the angle between their normals at that point and N_1, N_2 are the normals at $(2, -1, 2)$ to the given surfaces, therefore

$$N_1 \cdot N_2 = |N_1| |N_2| \cos \theta$$

$$\cos \theta = \frac{N_1 \cdot N_2}{|N_1| |N_2|} = \frac{(4\mathbf{i} - 2\mathbf{j} + 4\mathbf{k}) \cdot (4\mathbf{i} - 2\mathbf{j} - \mathbf{k})}{\sqrt{16+4+16} \sqrt{16+4+1}}$$

$$= \frac{16+4-4}{6 \cdot \sqrt{21}} = \frac{16}{6\sqrt{21}} = \frac{8}{3\sqrt{21}}$$

$$\theta = \cos^{-1} \left(\frac{8}{3\sqrt{21}} \right)$$

Ques) Find the values of a and b such that the surface $ax^2 - byz = (a+2)x$ and $4x^2y + z^3 = 4$ cut orthogonally at $(1, -1, 2)$ (3)

Soln - let

$$f_1 \equiv ax^2 - byz - (a+2)x = 0 \quad \text{--- (i)}$$

$$f_2 \equiv 4x^2y + z^3 - 4 = 0 \quad \text{--- (ii)}$$

$$\begin{aligned} \nabla f_1 &= \mathbf{i} \frac{\partial}{\partial x} (ax^2 - byz - (a+2)x) \\ &+ \mathbf{j} \frac{\partial}{\partial y} (ax^2 - byz - (a+2)x) \\ &+ \mathbf{k} \frac{\partial}{\partial z} (ax^2 - byz - (a+2)x) \end{aligned}$$

$$= \mathbf{i} (2ax - a - 2) + \mathbf{j} (-bz) + \mathbf{k} (-by)$$

$$\text{At } (1, -1, 2)$$

$$\nabla f_1 = (a-2)\mathbf{i} - 2b\mathbf{j} + bk \quad \text{--- (iii)}$$

$$\begin{aligned} \nabla f_2 &= \mathbf{i} \frac{\partial}{\partial x} (4x^2y + z^3 - 4) + \mathbf{j} \frac{\partial}{\partial y} (4x^2y + z^3 - 4) \\ &+ \mathbf{k} \frac{\partial}{\partial z} (4x^2y + z^3 - 4) \end{aligned}$$

$$= \mathbf{i} (8xy) + \mathbf{j} (4x^2) + \mathbf{k} (3z^2)$$

$$\text{At } (1, -1, 2)$$

$$\nabla f_2 = -8\mathbf{i} + 4\mathbf{j} + 12\mathbf{k}$$

The surface (i) and (ii) cut will cut orthogonally if $\nabla f_1 \cdot \nabla f_2 = 0$

$$\Rightarrow [(a-2)\mathbf{i} - 2b\mathbf{j} + b\mathbf{k}] \cdot [-8\mathbf{i} + 4\mathbf{j} + 12\mathbf{k}] = 0$$

$$\Rightarrow -8(a-2) - 8b + 12b = 0$$

$$\Rightarrow -8a + 16 + 4b = 0$$

$$\Rightarrow -8a - 2a + 4 + b = 0$$

$$\Rightarrow 2a - b = 4 \quad \text{--- (iv)}$$

Also, since the point $(1, -1, 2)$ lies on (i) and (ii), we have

$$\text{from (i)} \Rightarrow a + 2b - (a+2) = 0$$

$$\Rightarrow a + 2b - a - 2 = 0$$

$$\Rightarrow 2b = 2 \Rightarrow b = 1$$

$$\text{from (iv)} \Rightarrow 2a - 1 = 4$$

$$2a = 5$$

$$a = 5/2$$

$$\text{Hence } a = 5/2, b = 1$$

(4)

Que) Find $\text{div } F$ and $\text{curl } F$ where

$$F = \text{grad} (x^3 + y^3 + z^3 - 3xyz)$$

Soln:- $\text{grad} (x^3 + y^3 + z^3 - 3xyz) = \nabla (x^3 + y^3 + z^3 - 3xyz)$

$$= \mathbf{i} \frac{\partial}{\partial x} (x^3 + y^3 + z^3 - 3xyz) + \mathbf{j} \frac{\partial}{\partial y} (x^3 + y^3 + z^3 - 3xyz) + \mathbf{k} \frac{\partial}{\partial z} (x^3 + y^3 + z^3 - 3xyz)$$

$$= \mathbf{i} (3x^2 - 3yz) + \mathbf{j} (3y^2 - 3xz) + \mathbf{k} (3z^2 - 3xy)$$

$$+ \mathbf{k} (3z^2 - 3xy)$$

since $F = \text{grad} (x^3 + y^3 + z^3 - 3xyz)$

$$\therefore F = (3x^2 - 3yz)\mathbf{i} + (3y^2 - 3xz)\mathbf{j} + (3z^2 - 3xy)\mathbf{k}$$

$$\text{div } F = \nabla \cdot F$$

$$= \left(\mathbf{i} \frac{\partial}{\partial x} + \mathbf{j} \frac{\partial}{\partial y} + \mathbf{k} \frac{\partial}{\partial z} \right) \cdot \left\{ (3x^2 - 3yz)\mathbf{i} + (3y^2 - 3xz)\mathbf{j} + (3z^2 - 3xy)\mathbf{k} \right\}$$

$$= \frac{\partial}{\partial x} (3x^2 - 3yz) + \frac{\partial}{\partial y} (3y^2 - 3xz) + \frac{\partial}{\partial z} (3z^2 - 3xy)$$

$$= 6x + 6y + 6z = 6(x + y + z)$$

$$\text{Curl } F = \nabla \times F$$

$$= \begin{vmatrix} \mathbf{i} & \mathbf{j} & \mathbf{k} \\ \frac{\partial}{\partial x} & \frac{\partial}{\partial y} & \frac{\partial}{\partial z} \\ 3x^2-3yz & 3y^2-3xz & 3z^2-3xy \end{vmatrix}$$

$$= \mathbf{i}(-3x+3x) - \mathbf{j}(-3y+3y)$$

$$+ \mathbf{k}(-3z+3z)$$

$$= 0\mathbf{i} - \mathbf{j}(0) + \mathbf{k}(0) = 0$$

Que) If $f = (x^2+y^2+z^2)^{-n}$ find $\text{div grad } f$ and determine n if $\text{div grad } f = 0$

Soln

$$r = \sqrt{x^2+y^2+z^2}$$

$$r^2 = x^2+y^2+z^2$$

$$f = (x^2+y^2+z^2)^{-n} = (r^2)^{-n} = r^{-2n}$$

$$\text{grad } f = \sum \mathbf{i} \frac{\partial f}{\partial x} = \sum \mathbf{i} \frac{\partial}{\partial x} (r^{-2n})$$

$$= \sum \mathbf{i} (-2n) r^{-2n-1} \frac{\partial r}{\partial x}$$

$$= \sum \mathbf{i} (-2n) r^{-2n-1} \frac{x}{r}$$

$$= \sum \mathbf{i} (-2n) r^{-2n-2} x$$

(5)

$$= (-2n) r^{-2n-2} \Sigma x^2$$

$$= (-2n) r^{-2n-2} R \quad [\Sigma x^2 = R]$$

$$\cancel{\text{div grad } f} = \cancel{-\nabla \cdot \text{grad } f}$$

$$\text{div}(\text{grad } f) = \text{div}(-2n r^{-2n-2} R)$$

$$= (-2n) [\text{grad}(r^{-2n-2}) \cdot R + r^{-2n-2} \text{div } R]$$

$$= (-2n) \left[\Sigma (-2n-2) r^{-2n-3} \frac{\partial x}{\partial x} \cdot R + 3 r^{-2n-2} \right] \quad [\text{div } R = 3]$$

$$= (-2n) \left[\Sigma (-2n-2) r^{-2n-3} \frac{x}{r} \cdot R + 3 r^{-2n-2} \right]$$

$$= (-2n) \left[(-2n-2) r^{-2n-4} \Sigma x^2 \cdot R + 3 r^{-2n-2} \right]$$

$$= (-2n) \left[(-2n-2) r^{-2n-4} R \cdot R + 3 r^{-2n-2} \right]$$

$$= (-2n) \left[(-2n-2) r^{-2n-4} r^2 + 3 r^{-2n-2} \right] \quad [R \cdot R = r^2]$$

$$= (-2n) \left[(-2n-2) r^{-2n-2} + 3 r^{-2n-2} \right]$$

$$= (-2n) r^{-2n-2} [-2n-2 + 3]$$

$$= (2n) (2n-1) r^{-2n-2}$$

~~Suppose~~

Now if $\text{div grad } f = 0$

$$(2n)(2n-1)r^{-2n-2} = 0$$

$$\Rightarrow (2n-1) = 0$$

$$\Rightarrow n = 1/2$$

$$n \neq 0$$
$$r \neq 0$$

Que) Prove that

$$\nabla^2 f(r) = f''(r) + \frac{2}{r} f'(r)$$

Soln

$$\nabla^2 = \left(\frac{\partial^2}{\partial x^2} + \frac{\partial^2}{\partial y^2} + \frac{\partial^2}{\partial z^2} \right)$$

$$\nabla^2 f(r) = \left(\frac{\partial^2}{\partial x^2} + \frac{\partial^2}{\partial y^2} + \frac{\partial^2}{\partial z^2} \right) f(r)$$

$$= \frac{\partial^2}{\partial x^2} \{f(r)\} + \frac{\partial^2}{\partial y^2} \{f(r)\} + \frac{\partial^2}{\partial z^2} \{f(r)\}$$

— — (i)

Now $\frac{\partial}{\partial x} [f(r)] = f'(r) \frac{\partial r}{\partial x}$

$$\frac{\partial}{\partial x} [f(r)] = f'(r) \frac{x}{r}$$

$$\left(\frac{\partial r}{\partial x} = \frac{x}{r} \right)$$

$$= x \left(\frac{f'(r)}{r} \right)$$

(6)

$$\frac{\partial^2}{\partial x^2} =$$

$$\frac{\partial^2}{\partial x^2} f(x) = \frac{\partial}{\partial x} \left[\frac{\partial}{\partial x} f(x) \right]$$

$$= \frac{\partial}{\partial x} \left[x \frac{f'(x)}{x} \right]$$

$$= 1 \cdot \frac{f'(x)}{x} + x \left\{ \frac{x f''(x) - f'(x) \cdot 1}{x^2} \right\} \frac{\partial x}{\partial x}$$

$$= \frac{f'(x)}{x} + x \left\{ \frac{x f''(x) - f'(x)}{x^2} \right\} \frac{x}{x}$$

$$= \frac{f'(x)}{x} + \frac{x^2}{x^3} (x f''(x) - f'(x))$$

$$= \frac{f'(x)}{x} + \frac{x^2}{x^2} f''(x) - \frac{x^2}{x^3} f'(x) \quad \text{--- (2)}$$

Similarly

$$\frac{\partial^2}{\partial y^2} \{f(x)\} = \frac{f'(x)}{y} + \frac{y^2}{y^2} f''(x) - \frac{y^2}{y^3} f'(x) \quad \text{--- (3)}$$

$$\& \frac{\partial^2}{\partial z^2} [f(x)] = \frac{f'(x)}{z} + \frac{z^2}{z^2} f''(x) - \frac{z^2}{z^3} f'(x) \quad \text{--- (4)}$$

Adding ②, ③ & ④ we get

$$\frac{\partial^2}{\partial x^2} \{f(x)\} + \frac{\partial^2}{\partial y^2} \{f(x)\} + \frac{\partial^2}{\partial z^2} \{f(x)\}$$

$$= \frac{3 f'(x)}{x} + \frac{(x^2 + y^2 + z^2)}{x^2} f''(x)$$

$$- \frac{(x^2 + y^2 + z^2)}{x^3} f'(x)$$

$$= 3 \frac{f'(x)}{x} + \frac{x^2}{x^2} f''(x) - \frac{x^2}{x^3} f'(x)$$

$$= 3 \frac{f'(x)}{x} + f''(x) - \frac{1}{x} f'(x)$$

$$= \frac{2 f'(x)}{x} + f''(x)$$

$$\Rightarrow \nabla^2 f(x) = \frac{2 f'(x)}{x} + f''(x)$$

Hence proved.